feat: improve choice nodes + postpone

tests/lean/run/choiceExpectedTypeBug.lean
@@ -1,3 +1,5 @@
+import Lean
+
 new_frontend
 
 structure A :=
@@ -12,3 +14,32 @@ theorem ex : f = { x := 10 } :=
 rfl
 
 #check f
+
+syntax [emptyS] "⟨" "⟩"  : term -- overload `⟨ ⟩` notation
+
+open Lean
+open Lean.Elab
+open Lean.Elab.Term
+
+@[termElab emptyS] def elabEmptyS : TermElab :=
+fun stx expectedType? => do
+  tryPostponeIfNoneOrMVar expectedType?;
+  stxNew ← `(Nat.zero);
+  withMacroExpansion stx stxNew $ elabTerm stxNew expectedType?
+
+def foo (x : Unit) := x
+
+def f1 : Unit :=
+let x := ⟨ ⟩;
+foo x
+
+def f2 : Unit :=
+let x := ⟨ ⟩;
+x
+
+def f3 : Nat :=
+let x := ⟨ ⟩;
+x
+
+theorem ex2 : f3 = 0 :=
+rfl
