src/Lean/Elab/Term.lean
@@ -878,8 +878,8 @@ private partial def elabTermAux (expectedType? : Option Expr) (catchExPostpone :
 def elabTerm (stx : Syntax) (expectedType? : Option Expr) (catchExPostpone := true) : TermElabM Expr :=
 withRef stx $ elabTermAux expectedType? catchExPostpone true stx
 
-def elabTermEnsuringType (stx : Syntax) (expectedType? : Option Expr) : TermElabM Expr := do
-e ← elabTerm stx expectedType?;
+def elabTermEnsuringType (stx : Syntax) (expectedType? : Option Expr) (catchExPostpone := true) : TermElabM Expr := do
+e ← elabTerm stx expectedType? catchExPostpone;
 withRef stx $ ensureHasType expectedType? e
 
 def elabTermWithoutImplicitLambdas (stx : Syntax) (expectedType? : Option Expr) (catchExPostpone := true) : TermElabM Expr := do
